Harden ERC20 and WETH effect specs

src/generated/verity/WETHIface.sol
@@ -3,6 +3,7 @@
 pragma solidity ^0.8.20;
 
 interface WETHIface {
+    function decimals() external view returns (uint256);
     function totalSupply() external view returns (uint256);
     function balanceOf(address account) external view returns (uint256);
     function allowance(address ownerAddr, address spender) external view returns (uint256);
